## Homogeneous
For a 2nd order, linear homogeneous ODE with constant coefficients:
$$
a \frac{d^{2}y}{dx^{2}}+b \frac{dy}{dx}+cy=0
$$
Consider a solution of the form:
$$
y=Ae^{\lambda x}
$$
$$
\implies \frac{dy}{dx}=\lambda Ae^{\lambda x}
$$
$$
\implies \frac{d^{2}y}{dx^{2}}=\lambda^{2}Ae^{\lambda x}
$$
Substitute these back into the original equation
$$
a(\lambda^{2}Ae^{\lambda x} )+b(\lambda Ae^{\lambda x})+c(Ae^{\lambda x})=0
$$
$$
\implies Ae^{\lambda x}(a\lambda^{2}+b\lambda+c)=0
$$
So we get the auxiliary equation:
$$
a\lambda^{2}+b\lambda+c=0
$$
With solutions: $\lambda=\alpha$ and $\lambda=\beta$
$\therefore$ the general solution is the sum of these:
$$
y=Ae^{\alpha x}+Be^{\beta x}
$$
The particular solution can be found using initial conditions
## Repeated Roots
If $\alpha=\beta$, the general solution will instead be:
$$
y=(A+Bx)e^{\alpha x}
$$
Note that in this case the product rule will be needed to find the particular solution
## Complex Roots
If $\alpha,\beta \in \mathbb{C}$, $\alpha=\beta ^{*}$, ie. $\alpha=a+bi$, $\beta=a-bi$ and the general solution will be:
$$
y=Ae^{(a+bi)x}+Be^{(a-bi)x}=e^{a}(Ae^{bix}+Be^{-bix})
$$
$$
=e^{a}(A(\cos bx+i\sin bx)+B(\cos bx-i\sin bx))
$$
$$
=e^{a}((A+B)\cos bx+(A-B)i\sin bx)
$$
Which can be rewritten as:
$$
y=e^{a}(P\cos bx+Q\sin bx)
$$
Which is the new general solution which can then be rewritten in harmonic form:
$$
y=e^{a}R\cos(bx-\theta)
$$
Where $R=\sqrt{ P^{2}+Q^{2} }$ and $\theta=\arctan\left( \frac{Q}{P} \right)$
## Non-Homogeneous
For a 2nd order, linear non-homogeneous ODE with constant coefficients:
$$
a \frac{d^{2}y}{dx^{2}}+b \frac{dy}{dx}+cy=f(x)
$$
### General Form
If $y=y_{1}$ is a solution to:
$$
ay''+by'+cy=f(x)
$$
and $y=y_{2}$ is a solution to:
$$
ay''+by'+cy=0
$$
Then let 
$$
y=y_{1}+y_{2}
$$
$$
\implies y'=y_{1}'+y_{2}'
$$
$$
\implies y''=y_{1}''+y_{2}''
$$
$$
\implies a(y_{1}''+y_{2}'')+b(y_{1}'+y_{2}')+c(y_{1}+y_{2})
$$
$$
=(ay_{1}''+by_{1}'+cy_{1})+(ay_{2}''+by_{2}'+cy_{2})
$$
$$
=f(x)+0=f(x)
$$
So our general solution can be in the form $y=y_{1}+y_{2}$
### Complimentary Function
This is $y_{2}$ from above, always do this first, this is the same as with homogeneous:
$$
y=Ae^{\alpha x}+Be^{\beta x}
$$
### Particular Integral
This is $y_{1}$ from above, do this part second
#### f(x)=constant
Try $y=\alpha$
#### f(x)=linear
Try $y=\alpha x+\beta$
#### f(x)=quadratic
Try $y=\alpha x^{2}+\beta x+\gamma\implies y'=2\alpha x+\beta\implies y''=2\alpha$
$a(2\alpha)+b(2\alpha x+\beta )+c(\alpha x^2 + \beta x + \gamma )$
#### $f(x)$ = polynomial#
Try $y=\alpha_{0}+\alpha_{1}x+\alpha_{2}x^{2}+\dots+\alpha_{n}x^{n}$
