For a surface defined by $g(x,y,z)=c$, we define 
$$
grad(g)=\nabla(g)=\begin{pmatrix}
\frac{ \partial g }{ \partial x } \\ \frac{ \partial g }{ \partial y } \\ \frac{ \partial g }{ \partial z } 
\end{pmatrix}
$$
When evaluated at a point, $\nabla(g)$ gives us a normal vector to $g(x,y,z)=c$, which can then be used to find the tangent
If $g(x,y,z)=f(x,y)-z=0\implies z=f(x,y)$, then
$$
\nabla(g)=\begin{pmatrix}
\frac{ \partial f }{ \partial x } \\\frac{ \partial f }{ \partial y } \\-1
\end{pmatrix}
$$
#Mathematics