![[Oscillating Masses on Springs 2024-02-27 21.50.13.excalidraw]]
Consider a spring with spring constant $k$, the spring applies force $F_{0}$ to the mass
The mass $m$ in the first part is in equilibrium, so we can write:
$$
F_{0}=mg
$$
Then consider pulling down on the mass and then releasing it. It will oscillate vertically. Consider when the mass is at a displacement $x$ below its equilibrium position. The extension of the spring is increased by $x$, so the force $F(x)$ exerted by the spring on the mass is now given by
$$
F(x)=F_{0}+kx
$$
The resultant downward force is:
$$
F_{r es}=mg-F(x)=mg-F_{0}-kx=mg-mg-kx=-kx
$$
Hence we have [[Simple Harmonic Motion]], and thus we know $a=-\omega^{2}x$
Consider the force on the spring in equilibrium:
$$
F=-kx=-m\omega^{2}x
$$
$$
\implies k=m\omega^{2}
$$
$$
\implies \omega = \sqrt{ \frac{k}{m} }
$$
And since $T=\frac{2\pi}{\omega}$:
$$
T=2\pi \sqrt{ \frac{m}{k} }
$$
And since $f=\frac{1}{T}$
$$
f=\frac{1}{2\pi}\sqrt{ \frac{k}{m} }
$$
The same principle holds for a two-spring system
![[Oscillating Masses on Springs 2024-02-27 22.29.33.excalidraw]]
The same principle holds and the stiffness coefficient is simply the sum of the spring constants and there will again be SHM if friction is negligible

#Physics #Vibrations 