**


Consider the series
$$
\sum_{k=1}^{\infty} \frac{(-1)^{k+1}}{k}=c 
$$
Converges by the [[Alternating Series|alternating sign test]] with $c\in\left( \frac{1}{2},1 \right)$
Look at
$$
c=1-\frac{1}{2}-\frac{1}{4}+\frac{1}{3}-\frac{1}{6}-\frac{1}{8}+\frac{1}{5}-\frac{1}{10}-\frac{1}{12}+\dots
$$
i.e. an odd term followed by two even terms
$$
=\left( 1-\frac{1}{2} \right)-\frac{1}{4}+\left( \frac{1}{3}-\frac{1}{6} \right)-\frac{1}{8}+\left( \frac{1}{5}-\frac{1}{10} \right)-\frac{1}{12}+\dots 
$$
$$
= \frac{1}{2}-\frac{1}{4}+\frac{1}{6}-\frac{1}{8}+\frac{1}{10}-\frac{1}{12}+\dots 
$$
$$
= \frac{1}{2}\left( 1-\frac{1}{2}+\frac{1}{3}-\frac{1}{4}+\frac{1}{5}-\frac{1}{6}+\dots \right)=\frac{c}{2}
$$
Which links to the fact that commutativity does not work for infinite series
????